src/lib/communication/DY.Lib.Communication.Data.fst
@@ -1,0 +1,103 @@
+module DY.Lib.Communication.Data
+
+open Comparse
+open DY.Core
+open DY.Lib.Comparse.Glue
+open DY.Lib.Comparse.Parsers
+
+#set-options "--fuel 0 --ifuel 0 --z3cliopt 'smt.qi.eager_threshold=100'"
+
+(*** Messages ***)
+
+(**** Core ****)
+
+/// The following type is meant to be used to send a single byte with a function
+/// of the communication layer. Since the communication layer always takes a
+/// serializable data object we need to encapsulate the byte in a data object.
+[@@with_bytes bytes]
+type com_send_byte = {
+  b:bytes;
+}
+
+%splice [ps_com_send_byte] (gen_parser (`com_send_byte))
+%splice [ps_com_send_byte_is_well_formed] (gen_is_well_formed_lemma (`com_send_byte))
+
+instance parseable_serializeable_bytes_com_send_byte: parseable_serializeable bytes com_send_byte
+  = mk_parseable_serializeable ps_com_send_byte
+
+/// Data structure to return data from communication layer functions
+type communication_message (a:Type) = {
+  sender:principal;
+  receiver:principal;  
+  payload:a;
+}
+
+[@@with_bytes bytes]
+type signature_input = 
+  | Plain: sender:principal -> receiver:principal -> payload:bytes -> signature_input
+  | Encrypted: sender:principal -> receiver:principal -> payload:bytes -> pk:bytes -> signature_input
+
+#push-options "--ifuel 1 --fuel 0"
+%splice [ps_signature_input] (gen_parser (`signature_input))
+%splice [ps_signature_input_is_well_formed] (gen_is_well_formed_lemma (`signature_input))
+#pop-options
+
+instance parseable_serializeable_bytes_signature_input: parseable_serializeable bytes signature_input
+  = mk_parseable_serializeable ps_signature_input
+
+[@@with_bytes bytes]
+type signed_communication_message = {
+  msg:bytes;
+  signature:bytes;
+}
+
+%splice [ps_signed_communication_message] (gen_parser (`signed_communication_message))
+%splice [ps_signed_communication_message_is_well_formed] (gen_is_well_formed_lemma (`signed_communication_message))
+
+(**** Request/Response ****)
+
+[@@with_bytes bytes]
+type request_message = {
+  payload:bytes;
+  key:bytes
+}
+
+%splice [ps_request_message] (gen_parser (`request_message))
+%splice [ps_request_message_is_well_formed] (gen_is_well_formed_lemma (`request_message))
+
+[@@with_bytes bytes]
+type response_envelope = {
+  nonce:bytes;
+  ciphertext:bytes
+}
+
+%splice [ps_response_envelope] (gen_parser (`response_envelope))
+%splice [ps_response_envelope_is_well_formed] (gen_is_well_formed_lemma (`response_envelope))
+
+[@@with_bytes bytes]
+type authenticated_data = {
+  server:principal
+}
+
+%splice [ps_authenticated_data] (gen_parser (`authenticated_data))
+%splice [ps_authenticated_data_is_well_formed] (gen_is_well_formed_lemma (`authenticated_data))
+
+instance parseable_serializeable_bytes_authenticated_data: parseable_serializeable bytes authenticated_data
+  = mk_parseable_serializeable ps_authenticated_data
+
+
+(**** Message Type for all Messages on the Wire ****)
+
+[@@with_bytes bytes]
+type com_message_t =
+  | SigMessage: signed_communication_message -> com_message_t
+  | RequestMessage: request_message -> com_message_t
+  | ResponseMessage: response_envelope -> com_message_t
+
+#push-options "--ifuel 1"
+%splice [ps_com_message_t] (gen_parser (`com_message_t))
+%splice [ps_com_message_t_is_well_formed] (gen_is_well_formed_lemma (`com_message_t))
+#pop-options
+
+instance parseable_serializeable_bytes_com_message_t: parseable_serializeable bytes com_message_t
+  = mk_parseable_serializeable ps_com_message_t
